Veir/GlobalOpInfo.lean
@@ -35,6 +35,9 @@ match opCode with
 | .felt op => Felt.propertiesOf op
 | .string op => String_.propertiesOf op
 | .include op => Include_.propertiesOf op
+| .ram op => Ram.propertiesOf op
+| .cast op => Cast.propertiesOf op
+| .bool op => Bool_.propertiesOf op
 | .global op => Global.propertiesOf op
 | .function op => Function_.propertiesOf op
 
@@ -64,6 +67,9 @@ def OpCode.getEffects (opCode : OpCode) (props : _propertiesOf opCode) : MemoryE
   | .felt op, props => Felt.getEffects op props
   | .string op, props => String_.getEffects op props
   | .include op, props => Include_.getEffects op props
+  | .ram op, props => Ram.getEffects op props
+  | .cast op, props => Cast.getEffects op props
+  | .bool op, props => Bool_.getEffects op props
   | .global op, props => Global.getEffects op props
   | .function op, props => Function_.getEffects op props
 
@@ -91,6 +97,9 @@ def OpCode.getRegionKind (opCode : OpCode) (index : Nat) : RegionKind :=
   | .felt op => HasOpInfo.getRegionKind op index
   | .string op => HasOpInfo.getRegionKind op index
   | .include op => HasOpInfo.getRegionKind op index
+  | .ram op => HasOpInfo.getRegionKind op index
+  | .cast op => HasOpInfo.getRegionKind op index
+  | .bool op => HasOpInfo.getRegionKind op index
   | .global op => HasOpInfo.getRegionKind op index
   | .function op => HasOpInfo.getRegionKind op index
 
@@ -119,6 +128,9 @@ def OpCode.hasSSADominance (opCode : OpCode) (index : Nat) : Bool :=
   | .felt op => Felt.hasSSADominance op index
   | .string op => String_.hasSSADominance op index
   | .include op => Include_.hasSSADominance op index
+  | .ram op => Ram.hasSSADominance op index
+  | .cast op => Cast.hasSSADominance op index
+  | .bool op => Bool_.hasSSADominance op index
   | .global op => Global.hasSSADominance op index
   | .function op => Function_.hasSSADominance op index
 
@@ -148,6 +160,9 @@ def OpCode.hasNoTerminator (opCode : OpCode) (index : Nat) : Bool :=
   | .felt op => HasOpInfo.hasNoTerminator op index
   | .string op => HasOpInfo.hasNoTerminator op index
   | .include op => HasOpInfo.hasNoTerminator op index
+  | .ram op => HasOpInfo.hasNoTerminator op index
+  | .cast op => HasOpInfo.hasNoTerminator op index
+  | .bool op => HasOpInfo.hasNoTerminator op index
   | .global op => HasOpInfo.hasNoTerminator op index
   | .function op => HasOpInfo.hasNoTerminator op index
 
@@ -173,6 +188,9 @@ def OpCode.isIsolatedFromAbove (opCode : OpCode) : Bool :=
   | .felt op => HasOpInfo.isIsolatedFromAbove op
   | .string op => HasOpInfo.isIsolatedFromAbove op
   | .include op => HasOpInfo.isIsolatedFromAbove op
+  | .ram op => HasOpInfo.isIsolatedFromAbove op
+  | .cast op => HasOpInfo.isIsolatedFromAbove op
+  | .bool op => HasOpInfo.isIsolatedFromAbove op
   | .global op => HasOpInfo.isIsolatedFromAbove op
   | .function op => HasOpInfo.isIsolatedFromAbove op
 
@@ -202,6 +220,9 @@ def OpCode.isTerminator (opCode : OpCode) : Bool :=
   | .felt op => HasOpInfo.isTerminator op
   | .string op => HasOpInfo.isTerminator op
   | .include op => HasOpInfo.isTerminator op
+  | .ram op => HasOpInfo.isTerminator op
+  | .cast op => HasOpInfo.isTerminator op
+  | .bool op => HasOpInfo.isTerminator op
   | .global op => HasOpInfo.isTerminator op
   | .function op => HasOpInfo.isTerminator op
 
@@ -234,6 +255,9 @@ def OpCode.isConstantLike (opCode : OpCode) : Bool :=
   | .felt op => Felt.isConstantLike op
   | .string op => String_.isConstantLike op
   | .include op => Include_.isConstantLike op
+  | .ram op => Ram.isConstantLike op
+  | .cast op => Cast.isConstantLike op
+  | .bool op => Bool_.isConstantLike op
   | .global op => Global.isConstantLike op
   | .function op => Function_.isConstantLike op
 
@@ -262,6 +286,9 @@ def OpCode.propagatesPoison (opCode : OpCode) : Bool :=
   | .felt op => HasOpInfo.propagatesPoison op
   | .string op => HasOpInfo.propagatesPoison op
   | .include op => HasOpInfo.propagatesPoison op
+  | .ram op => HasOpInfo.propagatesPoison op
+  | .cast op => HasOpInfo.propagatesPoison op
+  | .bool op => HasOpInfo.propagatesPoison op
   | .global op => HasOpInfo.propagatesPoison op
   | .function op => HasOpInfo.propagatesPoison op
 
@@ -287,6 +314,9 @@ def Properties.fromAttrDict (opCode : OpCode) (attrDict : Std.HashMap ByteArray 
   | .felt op => Felt.fromAttrDict op attrDict
   | .string op => String_.fromAttrDict op attrDict
   | .include op => Include_.fromAttrDict op attrDict
+  | .ram op => Ram.fromAttrDict op attrDict
+  | .cast op => Cast.fromAttrDict op attrDict
+  | .bool op => Bool_.fromAttrDict op attrDict
   | .global op => Global.fromAttrDict op attrDict
   | .function op => Function_.fromAttrDict op attrDict
 
@@ -316,6 +346,9 @@ def Properties.toAttrDict
   | .felt op, props => Felt.toAttrDict op props
   | .string op, props => String_.toAttrDict op props
   | .include op, props => Include_.toAttrDict op props
+  | .ram op, props => Ram.toAttrDict op props
+  | .cast op, props => Cast.toAttrDict op props
+  | .bool op, props => Bool_.toAttrDict op props
   | .global op, props => Global.toAttrDict op props
   | .function op, props => Function_.toAttrDict op props
 
@@ -348,6 +381,9 @@ def OpCode.functionInterface? (opCode : OpCode) : Option (FunctionOpInterface (_
   | .felt op => HasOpInfo.functionInterface? op
   | .string op => HasOpInfo.functionInterface? op
   | .include op => HasOpInfo.functionInterface? op
+  | .ram op => HasOpInfo.functionInterface? op
+  | .cast op => HasOpInfo.functionInterface? op
+  | .bool op => HasOpInfo.functionInterface? op
   | .global op => HasOpInfo.functionInterface? op
   | .function op => HasOpInfo.functionInterface? op
 
@@ -376,6 +412,9 @@ def OpCode.verifyLocalInvariants (opCode : OpCode) (op : OperationPtr)
   | .felt opType => Felt.verifyLocalInvariants opType op ctx opIn
   | .string opType => String_.verifyLocalInvariants opType op ctx opIn
   | .include opType => Include_.verifyLocalInvariants opType op ctx opIn
+  | .ram opType => Ram.verifyLocalInvariants opType op ctx opIn
+  | .cast opType => Cast.verifyLocalInvariants opType op ctx opIn
+  | .bool opType => Bool_.verifyLocalInvariants opType op ctx opIn
   | .global opType => Global.verifyLocalInvariants opType op ctx opIn
   | .function opType => Function_.verifyLocalInvariants opType op ctx opIn
 
@@ -411,7 +450,8 @@ def OpCode.materializeConstant (opCode : OpCode) (value : RuntimeValue)
     -- fails to compile until it decides how, or whether, to materialize.
     | .riscv_cf _ | .riscv_stack _ | .rv64 _ | .cf _ | .builtin _
     | .verif _
-    | .func _ | .datapath _ | .pdl _ | .test _ | .string _ | .include _ | .global _
+    | .func _ | .datapath _ | .pdl _ | .test _ | .string _ | .include _ | .ram _ | .cast _
+    | .bool _ | .global _
     | .function _ => none
   guard materialized.fst.isConstantLike
   return materialized
