Test/LLZK/Bool/invalid.mlir
@@ -1,0 +1,10 @@
+// RUN: not veir-opt %s 2>&1 | filecheck %s
+
+// CHECK: Error verifying input program: bool.assert: Expected 0 result(s)
+"builtin.module"() ({
+  "function.def"() <{sym_name = "invalid_bool", function_type = (i1) -> ()}> ({
+^bb0(%a: i1):
+  %0 = "bool.assert"(%a) : (i1) -> i1
+  "function.return"() : () -> ()
+  }) {function.allow_non_native_field_ops} : () -> ()
+}) : () -> ()
